Refactor max example.

src/dafny/yul-bytecode-verif/max/max.dfy
@@ -19,54 +19,27 @@ include "../../Yul/Semantics.dfy"
 include "../../Yul/StrictSemantics.dfy"
 include "../../Yul/State.dfy"
 
+include "./max-bytecode.dfy"
+
 /**
   *  
   */
 module MaxBytecodeVerification {
 
   import opened Int
-  import opened YulSem = YulStrict
+  import opened YulStrict
   import opened YulState
-  import opened Opcode
-  import EvmState
-  import Memory
-  import EVM
-  import opened Bytecode
-  import Gas
+  import ByteUtils
+  import opened MaxBytecode
 
   /**
-    *  The labels (JUMPDEST) in the bytecode.
+    *   A ghost (verification-only) function.
     */
-  const tag_1: u8 := 0x0f
-  const tag_2: u8 := 0x0a
-  const tag_3: u8 := 0x1b
-  const tag_4: u8 := 0x18
-
-  /**
-    *  When a JUMP or JUMPI is executed we need to make sure the target location 
-    *  is a JUMPDEST.
-    *  This axiom enforces it.
-    */
-  lemma {:axiom} ValidJumpDest(s: EvmState.ExecutingState)
-    ensures s.IsJumpDest(tag_1 as u256)
-    ensures s.IsJumpDest(tag_2 as u256)
-    ensures s.IsJumpDest(tag_3 as u256)
-    ensures s.IsJumpDest(tag_4 as u256)
-
-  /**
-    *  Translation of the of the Yul code in Dafny.
-    *   Use Dafny native operators.
-    */
-  method Max(x: u256, y: u256, s: Executing) returns (result: u256, s': State)
-    ensures result == x || result == y
-    ensures result >= x && result >= y
-    ensures s' == s
+  ghost function maxu256(x: u256, y: u256): (r: u256)
+    ensures r == x || r == y
+    ensures r >= x && r >= y
   {
-    s' := s;
-    result := x;
-    if YulSem.Lt(x, y) {
-      result := y;
-    }
+    if x <= y then y else x
   }
 
   /**
@@ -93,6 +66,7 @@ module MaxBytecodeVerification {
     requires st.Capacity() >= 2
     requires st.evm.memory == s.yul.memory
 
+    ensures result == maxu256(x, y)
     ensures st'.EXECUTING?
     ensures st'.PC() == tag_2 as nat
     ensures st'.Operands() == st.Operands() - 2
@@ -112,21 +86,6 @@ module MaxBytecodeVerification {
   }
 
   /**
-    *  Translation of Yul code in Dafny.
-    */
-  method Main(s: Executing) returns (s': State)
-    requires s.MemSize() % 32 == 0
-    ensures s'.EXECUTING?
-    ensures s'.MemSize() > 0x40 + 31
-    ensures s'.Read(0x40) == 8
-  {
-    var x := 8;                     //  let
-    var y := 3;                     //  let
-    var z, s1 := Max(x, y, s);      //  funcall
-    s' := YulSem.MStore(0x40, z, s1);      //  memory store
-  }
-
-  /**
     *  Proof of simulation for Main.
     */
   method MainProof(s:  Executing, ghost st: EvmState.ExecutingState) returns (z': u256, s': State, ghost st': EvmState.State)
@@ -136,169 +95,26 @@ module MaxBytecodeVerification {
     requires s.MemSize() % 32 == 0
     requires st.evm.memory == s.yul.memory
 
-    ensures s'.EXECUTING?
-    ensures st'.EXECUTING?
-    ensures s'.MemSize() > 0x40 + 31
-    ensures s'.Read(0x40) == z'
-    ensures st'.evm.memory == s'.yul.memory
+    ensures s'.RETURNS?
+    ensures st'.RETURNS?
+    ensures s'.data == st'.data
+    ensures ByteUtils.ReadUint256(s'.data, 0) == 8
+    ensures ByteUtils.ReadUint256(st'.data, 0) == 8
   {
     ValidJumpDest(st);
     ghost var st1 := ExecuteFromZero(st);        //  bytecode move
-    var x := 8;                                 //  Yul move
-    var y := 3;                                 //  Yul move
-
+    var x := 8;                                  //  Yul move
+    var y := 3;                                  //  Yul move
+    assert st1.EXECUTING?;
     var z, s1, st2 := MaxProof(x, y, s, st1);    //  Simulation of call to Max.
+
     assert z == st2.Peek(0);
     assert s1 == s;
 
-    st' := ExecuteFromTag2(st2);          //  Bytecode move
-    z':= z;                             //  Yul move
-    s' := YulSem.MStore(0x40, z, s1);          //  Yul move
-  }
-
-  /**
-    *  Code starting at PC == 0.
-    */
-  function ExecuteFromZero(st: EvmState.ExecutingState): (s': EvmState.State)
-    requires st.Capacity() >= 5
-    requires st.Operands() >= 0
-    requires st.PC() == 0 as nat
-
-    ensures s'.EXECUTING?
-    ensures s'.PC() == tag_1 as nat
-  {
-    /*
-    00000000: PUSH1 0xa     //  tag_2 
-    00000002: PUSH1 0x8
-    00000004: PUSH1 0x3
-    00000006: SWAP1
-    00000007: PUSH1 0xf     //  tag_1 
-    00000009: JUMP
-    */
-    ValidJumpDest(st);
-    var s1 := Push1(st, tag_2);
-    var s2 := Push1(s1, 0x08);
-    var s3 := Push1(s2, 0x03);
-    var s4 := Swap(s3, 1);
-    assert s4.Peek(2) == tag_2 as u256;
-    var s5 := Push1(s4, tag_1);
-    assert s5.Peek(3) == tag_2 as u256;
-    var s6 := Jump(s5);
-    s6
-  }
-
-  function ExecuteFromTag2(st: EvmState.ExecutingState): (s': EvmState.State)
-    requires st.Capacity() >= 1
-    requires st.Operands() >= 0
-    requires st.PC() == tag_2 as nat
-  {
-    /*
-    0000000a: JUMPDEST
-    0000000b: PUSH1 0x40
-    0000000d: MSTORE
-    0000000e: STOP
-    */
-    var s1 := JumpDest(st);
-    var s2 := Push1(s1, 0x40);
-    var s3 := Bytecode.MStore(s2);
-    s3
-  }
-
-  function ExecuteFromTag1(st: EvmState.ExecutingState): (s': EvmState.State)
-    requires st.Capacity() >= 2
-    requires st.Operands() >= 3
-    requires st.PC() == tag_1 as nat
-    requires st.IsJumpDest(st.Peek(2))
-    requires st.Peek(2) == tag_2 as u256
-
-    ensures s'.EXECUTING?
-    ensures s'.Operands() == st.Operands()
-    ensures s'.Peek(0) == st.Peek(1)
-    ensures s'.Peek(1) == st.Peek(2)
-    ensures s'.Peek(2) == st.Peek(0)
-    ensures s'.PC() == if st.Peek(0) < st.Peek(1) then tag_3 as nat else tag_4 as nat
-  {
-    /*
-    0000000f: JUMPDEST      //  tag_1 
-    00000010: SWAP2
-    00000011: SWAP1
-    00000012: DUP1 
-    00000013: DUP4
-    00000014: LT
-    00000015: PUSH1 0x1b
-    00000017: JUMPI
-    */
-    ValidJumpDest(st);
-    var s1 := JumpDest(st); //  r, y, x
-    var s2 := Swap(s1, 2);  //  x, y, r
-    var s3 := Swap(s2, 1);  //  x, r, y
-    var s4 := Dup(s3, 1);   //  x, r, y, y
-    var s5 := Dup(s4, 4);   //  x, r, y, y, x
-    assert s5.PC() == 0x14;
-    var s6 := Bytecode.Lt(s5);       //  x, r, y, x < y
-    var s7 := Push1(s6, tag_3); //  x, r, y, x < y, tag_ 3
-    var s8 := JumpI(s7);        //  x, r, y
-    s8
-  }
-
-  function ExecuteFromTag4(st: EvmState.ExecutingState): (s': EvmState.State)
-    requires st.Operands() >= 3
-    requires st.PC() == tag_4 as nat
-    requires st.IsJumpDest(st.Peek(1))
-    requires st.Peek(1) as nat == tag_2 as nat
-
-    ensures s'.EXECUTING?
-    ensures s'.PC() == st.Peek(1) as nat == tag_2 as nat
-    ensures s'.Operands() == st.Operands() - 2
-    ensures s'.Peek(0) == st.Peek(2)
-  {
-    /*
-    00000018: JUMPDEST      // tag_4 x2, x1, x0 
-    00000019: POP           //  x2, x1 
-    0000001a: JUMP          //  x2 
-    */
-    var s9 := JumpDest(st);
-    var s10 := Pop(s9);
-    assert s10.IsJumpDest(s10.Peek(0));
-    var s11 := Jump(s10);
-    assert s11.PC() == st.Peek(1) as nat;
-    s11
-  }
-
-  function ExecuteFromTag3(st: EvmState.ExecutingState): (s': EvmState.State)
-    requires st.Operands() >= 3
-    requires st.Capacity() >= 1
-    requires st.PC() == tag_3 as nat
-    requires st.IsJumpDest(st.Peek(1))
-    requires st.Peek(1) == tag_2 as u256
-
-    ensures s'.EXECUTING?
-    ensures s'.PC() == tag_4 as nat
-    ensures s'.Operands() == st.Operands()
-  {
-    /*
-    0000001b: JUMPDEST      //  tag_ 3  x2, x1, x0 
-    0000001c: SWAP1         //  x2, x0, x1 
-    0000001d: SWAP2         //  x1, x0, x2 
-    0000001e: POP           //  x1, x0 
-    0000001f: SWAP1         //  x0, x1 
-    00000020: PUSH0         //  x0, x1, 0 
-    00000021: PUSH1 0x18    //  x0, x1, 0, 0x18 
-    00000023: JUMP          //  x0, x1, 0
-    */
-    ValidJumpDest(st);
-
-    var s1 := JumpDest(st);
-    var s2 := Swap(s1, 1);
-    var s3 := Swap(s2, 2);
-    var s4 := Pop(s3);
-    var s5 := Swap(s4, 1);
-    var s6 := Push0(s5);
-    var s7 := Push1(s6, tag_4);
-
-    var s8 := Jump(s7);
-    assert s8.Peek(0) == 0; //  x0, x1, 0
-    s8
+    st' := ExecuteFromTag2(st2);                //  Bytecode move
+    z':= z;                                     //  Yul move
+    var s2 := MStore(0x40, z, s1);              //  Yul move
+    s' := Return(0x40, 32, s2);                 //  Yul move
   }
 
   method {:main} Runner() {
